Snapshot

Monads.lean
@@ -15,4 +15,67 @@ theorem ul' (m : Type u → Type v) [Monad m] : unit_left m -> unit_left' m := b
   exact congrFun (h (f := f)) x
 
 theorem ul (m : Type u → Type v) [Monad m] : unit_left' m -> unit_left m := by
+  intro h
+  rw [unit_left'] at h
+  rw [unit_left]
+  intro α β f
+  funext a
+  specialize h (α := α) (β := β) (f := f)
+  have h' := congrFun h a
+  rw [Bind.kleisliRight] at h'
+  assumption
+
+def unit_right (m : Type u → Type v) [Monad m] :=
+  ∀ {α β : Type u}, ∀ {f : α -> m β}, (fun a => f a >>= pure) = f
+  -- or (f · >>= pure) = f
+
+def unit_right' (m : Type u → Type v) [Monad m] :=
+  ∀ {α β : Type u}, ∀ {f : α -> m β}, f >=> pure = f
+
+def ur' (m : Type u → Type v) [Monad m] : unit_right m -> unit_right' m := by
+  intro h
+  rw [unit_right] at h
+  rw [unit_right']
+  intro α β f
+  specialize h (α := α) (β := β) (f := f)
+  apply funext -- or ext x
+  intro x
+  rw [Bind.kleisliRight]
+  revert x
+  apply congrFun
+  assumption
+
+def ur (m : Type u → Type v) [Monad m] : unit_right' m -> unit_right m := by
+  rw [unit_right, unit_right']
+  intro h
+  intro α β f
+  specialize h (α := α) (β := β) (f := f)
+  have h' := congrFun h
+  simp [Bind.kleisliRight] at h' -- rw wouldn't work here *directly*
+  funext a
+  exact h' a
+
+def assoc (m : Type u -> Type v) [Monad m] :=
+  ∀ {α β γ : Type u} {f : α -> m β} {g : β → m γ},
+  ∀ (ma : m α), (ma >>= f >>= g) = (ma >>= fun a => f a >>= g)
+
+def assoc' (m : Type u -> Type v) [Monad m] :=
+  ∀ {α β γ δ: Type u} {f : α -> m β} {g : β → m γ} {h : γ -> m δ},
+  (f >=> g) >=> h = f >=> (g >=> h)
+
+theorem ass' (m : Type u -> Type v) [Monad m] : assoc m -> assoc' m := by
+  intro ha
+  rw [assoc, assoc'] at *
+  intro α β γ δ f g h
+  ext ma
+  simp [Bind.kleisliRight] -- ⊢ f ma >>= g >>= h = f ma >>= (g >=> h)
+  -- need to replace g >=> h with (fun x => (g >=> h) x) in order to
+  -- get rid of the Kleisli operator.
+  -- nth_rewrite would work, but that's in Mathlib
+  change f ma >>= g >>= h = f ma >>= (fun x => (g >=> h) x)
+  specialize ha (f := g) (g := h) (f ma)
+  simp [Bind.kleisliRight]
+  assumption
+
+theorem ass (m : Type u -> Type v) [Monad m] : assoc' m -> assoc m := by
   admit
